PotentialMethod.thy
@@ -1,5 +1,5 @@
 theory PotentialMethod
-imports QuantSepCon
+imports QuantSepConState
 begin
 
 
@@ -15,6 +15,7 @@ typedef 'a dual_ord = "UNIV :: 'a set" morphisms of_dual_ord to_dual_ord
   by auto
 
 setup_lifting type_definition_dual_ord
+print_theorems
 
 instantiation dual_ord :: (ord) ord
 begin
@@ -160,16 +161,138 @@ interpretation ENNREAL_PLUS: quant_sep_con "(+)" "0::ennreal dual_ord" "(-)"
   subgoal by (auto simp add: bot_ennreal minus_top_ennreal) 
   done
 
+term of_dual_ord
+
+definition star_pot_method (infixr "\<star>\<^sub>p" 35) where
+  "star_pot_method == (\<lambda>P Q x. of_dual_ord (ENNREAL_PLUS.sep_conj_s_q (\<lambda>x. to_dual_ord (P x)) (\<lambda>x. to_dual_ord (Q x)) x))"
+
+definition wand_pot_method (infixr "-\<star>\<^sub>p" 35) where
+  "wand_pot_method == (\<lambda>P Q x. of_dual_ord (ENNREAL_PLUS.sep_impl_s_q (\<lambda>x. to_dual_ord (P x)) (\<lambda>x. to_dual_ord (Q x)) x))"
 
 
-abbreviation star_pot_method (infixl "**\<^sub>p" 60) where
-  "star_pot_method == ENNREAL_PLUS.sep_conj_q"
+context 
+  includes lifting_syntax
+begin
+  
 
-abbreviation wand_pot_method (infixl "-*\<^sub>p" 60) where
-  "wand_pot_method == ENNREAL_PLUS.sep_impl_qq"
+lemma [transfer_rule]:   "((rel_prod (=) (=) ===> pcr_dual_ord (=))
+             ===> ((rel_prod (=) (=) ===> pcr_dual_ord (=))
+               ===> rel_prod (=) (=) ===> pcr_dual_ord (=)))
+           (\<star>\<^sub>p) ENNREAL_PLUS.sep_conj_s_q"
+  apply (auto simp: rel_fun_def pcr_dual_ord_def OO_def star_pot_method_def  cr_dual_ord_def 
+                   )
+  apply(rule arg_cong[where f=of_dual_ord])
+proof (goal_cases)
+  case (1 x y xa ya a b)
+  have "ENNREAL_PLUS.sep_conj_s_q (\<lambda>xa. to_dual_ord (x xa)) (\<lambda>x. to_dual_ord (xa x)) (a, b)
+        = ENNREAL_PLUS.sep_conj_s_q (\<lambda>xa. to_dual_ord (x (fst xa, snd xa))) (\<lambda>x. to_dual_ord (xa (fst x, snd x))) (a, b)"
+    by auto
+  also have "\<dots> = ENNREAL_PLUS.sep_conj_s_q (\<lambda>xa. to_dual_ord (of_dual_ord (y (fst xa, snd xa))))
+                           (\<lambda>x. to_dual_ord (xa (fst x, snd x))) (a, b)"
+    using 1(1) by metis
+  also have "\<dots> = ENNREAL_PLUS.sep_conj_s_q (\<lambda>xa. to_dual_ord (of_dual_ord (y (fst xa, snd xa))))
+                           (\<lambda>x. to_dual_ord (of_dual_ord (ya (fst x, snd x)))) (a, b)"
+    using 1(2) by metis
+  also have "\<dots> = ENNREAL_PLUS.sep_conj_s_q y ya (a, b)"
+    apply(subst dual_ord.of_dual_ord_inverse)
+    apply(subst dual_ord.of_dual_ord_inverse)  by auto 
+  finally show ?case .
+qed 
 
 
-thm ENNREAL_PLUS.adjoint_general
+term "(\<star>\<^sub>p)"
+term "pcr_dual_ord (=)"
+term "rel_prod (=) (=)"
+term "rel_fun"
+term " (rel_prod (=) (=) ===> pcr_dual_ord (=))"
+
+end
+term cr_dual_ord
+term pcr_dual_ord
+
+
+definition "sep_empty_s\<^sub>p \<equiv> (%sh. of_dual_ord (ENNREAL_PLUS.sep_empty_s_q sh))" 
+definition "emb\<^sub>p \<equiv> (\<lambda>P sh. of_dual_ord (ENNREAL_PLUS.emb P sh))" 
+
+lemma star_pot_method_alt:
+  "(P \<star>\<^sub>p Q) = (\<lambda>(s,h). Inf { P(s,x) + Q(s,y) | x y. h=x+y \<and> x ## y})"
+  unfolding ENNREAL_PLUS.sep_conj_s_q_def
+        ENNREAL_PLUS.sep_conj_q_def star_pot_method_def by transfer auto
+
+lemma wand_pot_method_alt:
+  "(P -\<star>\<^sub>p Q) = (\<lambda>(s,h). SUP h': { h'. h ## h' \<and> (bot < P(s,h') \<or> bot < Q(s,h+h') )
+                                \<and> ( P(s,h') < top \<or> Q(s,h+h') < top)}. 
+                                    (Q (s,h + h')) - P (s,h') )"
+  unfolding ENNREAL_PLUS.sep_impl_qq_def ENNREAL_PLUS.sep_impl_s_q_def wand_pot_method_def
+  apply(transfer) apply (rule ext) apply auto by metis
+
+lemma sep_empty_s\<^sub>e_def: "sep_empty_s\<^sub>p = (\<lambda>(s, h). emb\<^sub>p (\<lambda>h. h = 0) h)"
+  by (auto simp: sep_empty_s\<^sub>p_def emb\<^sub>p_def ENNREAL_PLUS.sep_empty_s_q_def
+                    ENNREAL_PLUS.sep_empty_q_def  )
+
+ 
+
+lemma 
+  fixes X :: "_ * 'a::{sep_algebra} \<Rightarrow> ennreal"
+  shows "(X \<star>\<^sub>p Y) = (Y \<star>\<^sub>p X)"
+  apply(rule ext)
+  apply transfer oops
+thm ENNREAL_PLUS.sep_conj_s_q_commute
+thm ENNREAL_PLUS.sep_conj_s_q_neutral
+thm ENNREAL_PLUS.sep_conj_s_q_assoc
+thm ENNREAL_PLUS.sep_conj_q_left_commute_s
+
+thm ENNREAL_PLUS.sep_conj_q_s_c
+
+
+lemma theorem_3_6_s:
+  fixes P Q R :: "(_ \<times> 'a::{sep_algebra} \<Rightarrow> ennreal)"
+  shows 
+  "(P \<star>\<^sub>p sup Q R) = (\<lambda>s. sup ((P \<star>\<^sub>p Q) s) ((P \<star>\<^sub>p R) s))"
+  (*  "(P \<star> (\<lambda>s. Q s + R s)) \<le> (\<lambda>s. (P \<star> Q) s + (P \<star> R) s)" *)
+  "( (emb\<^sub>p \<phi>) \<star>\<^sub>p (Q + R)) \<le> ((emb\<^sub>p \<phi>) \<star>\<^sub>p Q) + ((emb\<^sub>p \<phi>) \<star>\<^sub>p R)"
+(*  subgoal using Exp.theorem_3_6_s(1) .
+  subgoal
+    apply(subst (1) times_fun')    
+    using Exp.theorem_3_6_s(2)
+    by (auto simp: le_fun_def)
+  done *) oops
+
+thm ENNREAL_PLUS.sep_impl_s_q_mono
+thm ENNREAL_PLUS.sep_conj_s_q_mono'
+
+lemma adjoint_general_s:
+  shows "(X \<star>\<^sub>p P) \<ge> Y \<longleftrightarrow> X \<ge> (P -\<star>\<^sub>p Y)" 
+  using ENNREAL_PLUS.adjoint_general_s oops
+
+
+lemma quant_modus_ponens_general_s:
+  shows "( P \<star>\<^sub>p (P -\<star>\<^sub>p X)) \<le> X"
+  using ENNREAL_PLUS.quant_modus_ponens_general_s oops
+
+
+definition "pure\<^sub>p \<equiv> (\<lambda>P.  (ENNREAL_PLUS.pure_q (\<lambda>sh. to_dual_ord (P sh))))"
+
+lemma wrap: "\<forall>s h1 h2. to_dual_ord (X (s, h1)) = to_dual_ord (X (s, h2))
+    \<Longrightarrow> \<forall>s h1 h2. of_dual_ord (to_dual_ord (X (s, h1))) = of_dual_ord (to_dual_ord (X (s, h2)))"
+  by metis
+
+lemma pure\<^sub>e_alt: "pure\<^sub>p X \<longleftrightarrow> (\<forall>s h1 h2. X (s,h1) = X (s,h2))"
+  unfolding pure\<^sub>p_def ENNREAL_PLUS.pure_q_def apply auto
+  subgoal by(auto dest: wrap simp add: dual_ord.to_dual_ord_inverse)  
+  subgoal by metis
+  done
+
+lemma  theorem_3_11_1: "pure\<^sub>p X \<Longrightarrow> X + Y \<le> (X \<star>\<^sub>p Y)"
+    apply(subst (1) times_fun')   
+  using ENNREAL_PLUS.theorem_3_11_1 oops
+
+lemma theorem_3_11_3:
+  "pure\<^sub>p X \<Longrightarrow> ((X + Y) \<star>\<^sub>p Z) = X + (Y \<star>\<^sub>p Z)"
+    apply(subst times_fun')+
+  using ENNREAL_PLUS.theorem_3_11_3 oops
+  
+ 
 
 
 (* TODO: maybe transfer back *)
